theories/rules/rules_JmpIEpcc.v
@@ -1,0 +1,612 @@
+From iris.base_logic Require Export invariants gen_heap.
+From iris.program_logic Require Export weakestpre ectx_lifting.
+From iris.proofmode Require Import proofmode.
+From iris.algebra Require Import frac.
+From cap_machine Require Export rules_base register_tactics.
+
+Section cap_lang_rules.
+  Context `{memG Σ, regG Σ}.
+  Context `{MachineParameters}.
+  Implicit Types P Q : iProp Σ.
+  Implicit Types σ : ExecConf.
+  Implicit Types c : cap_lang.expr.
+  Implicit Types a b : Addr.
+  Implicit Types r : RegName.
+  Implicit Types v : cap_lang.val.
+  Implicit Types w : Word.
+  Implicit Types reg : gmap RegName Word.
+  Implicit Types ms : gmap Addr Word.
+
+  Inductive Jmp_failure (regs: Reg) (r: RegName) (mem : gmap Addr Word) :=
+  | Jmp_fail_not_IEpcc w :
+      regs !! r = Some w ->
+      is_iepcc_cap w = false ->
+      Jmp_failure regs r mem
+  | Jmp_fail_bounds b e a :
+      regs !! r = Some (WCap IEpcc b e a) ->
+      not (b < e)%a ->
+      Jmp_failure regs r mem
+  .
+
+  Inductive Jmp_spec
+    (regs: Reg) (r: RegName)
+    (regs': Reg) (mem : gmap Addr Word) : cap_lang.val → Prop
+  :=
+  | Jmp_spec_success_IEpcc b e a wpc :
+    regs !! r = Some (WCap IEpcc b e a) ->
+    (b < e)%a ->
+    mem !! b = Some wpc ->
+    regs' = ( <[ idc := (WCap RW b e a) ]> (<[ PC := wpc ]> regs)) ->
+    Jmp_spec regs r regs' mem NextIV
+
+  | Jmp_spec_failure :
+    Jmp_failure regs r mem ->
+    regs' = regs ->
+    Jmp_spec regs r regs' mem FailedV.
+
+
+  Definition reg_allows_IEpcc_jmp (regs : Reg) (r : RegName) p b e a :=
+    regs !! r = Some (WCap p b e a)
+    /\ p = IEpcc
+    ∧ (b < e)%a.
+
+  Lemma contra_reg_allows_IEpcc_jmp r regs b e a :
+    regs !! r = Some (WCap IEpcc b e a) ->
+    (b < e)%a ->
+    ¬ reg_allows_IEpcc_jmp regs r IEpcc b e a ->
+    False.
+  Proof.
+    intros Hreg Hwb Hdec1.
+    apply not_and_r in Hdec1 as [Hcontra|Hcontra]; simplify_eq.
+    apply Hcontra ; repeat (split ; auto).
+  Qed.
+
+  Lemma reg_allows_IEpcc_jmp_same
+    (regs : Reg) (r : RegName)
+    (p p' : Perm) (b b' e e' a a' : Addr):
+    reg_allows_IEpcc_jmp regs r p b e a ->
+    regs !! r = Some (WCap p' b' e' a') ->
+    (p = p' /\ b = b' /\ e = e' /\ a = a').
+  Proof.
+    intros HallowJmp Hregs.
+    destruct HallowJmp as (Hregs'&->&_).
+    by rewrite Hregs' in Hregs; simplify_eq.
+  Qed.
+
+  (* NOTE: cond is a condition to re-use the setup with rules_Jnz.v *)
+  Definition allow_jmp_mmap_or_true (cond : Prop) `{Decision cond} (r : RegName) (regs : Reg) (mem : Mem) :=
+    ∃ p b e a, read_reg_inr regs r p b e a ∧
+                 if decide (reg_allows_IEpcc_jmp regs r p b e a /\ cond) then
+                   ∃ w, mem !! b = Some w
+                 else True.
+
+  Definition allow_jmp_rmap_or_true (cond : Prop) `{Decision cond}  (r : RegName) (regs : Reg) :=
+    ∃ p b e a, read_reg_inr regs r p b e a ∧
+                 if decide (reg_allows_IEpcc_jmp regs r p b e a /\ cond) then
+                   ∃ widc, regs !! idc = Some widc
+                 else True.
+
+  Lemma allow_jmp_mmap_or_true_not_ie (cond : Prop) `{Decision cond}  (r : RegName) (regs : Reg) (mem : Mem) (w : Word) :
+    is_iepcc_cap w = false ->
+    regs !! r = Some w ->
+    allow_jmp_mmap_or_true cond r regs mem.
+  Proof.
+    intros Hvpc.
+    destruct_word w; eauto; eexists _,_,_,_; split
+    ;try (rewrite /read_reg_inr ; simplify_map_eq; auto).
+    rewrite /reg_allows_IEpcc_jmp ; simplify_map_eq ; auto.
+    all: case_decide as Heq ; simplify_eq ; auto.
+    all: try destruct Heq as [(? & -> & ? ) ?] ; simplify_map_eq.
+    all: try destruct Heq as [(? & _) ?] ; simplify_map_eq.
+    Unshelve. all: try exact O; try exact 0%a.
+  Qed.
+
+  Lemma allow_jmp_rmap_or_true_not_ie (cond : Prop) `{Decision cond}  (r : RegName) (regs : Reg) (w : Word) :
+    is_iepcc_cap w = false ->
+    regs !! r = Some w ->
+    allow_jmp_rmap_or_true cond r regs.
+  Proof.
+    intros Hvpc.
+    destruct_word w; eauto; eexists _,_,_,_; split
+    ;try (rewrite /read_reg_inr ; simplify_map_eq; auto).
+    rewrite /reg_allows_IEpcc_jmp ; simplify_map_eq ; auto.
+    all: case_decide as Heq ; simplify_eq ; auto.
+    all: try destruct Heq as [(? & -> & ? ) ?] ; simplify_map_eq.
+    all: try destruct Heq as [(? & _) ?] ; simplify_map_eq.
+    Unshelve. all: try exact O; try exact 0%a.
+  Qed.
+
+
+  Lemma allow_jmp_mmap_or_true_ie (cond : Prop) `{Decision cond}
+    (r : RegName) (regs : Reg) (mem : Mem)
+    (b e a : Addr) (widc wa wa' : Word) :
+    regs !! r = Some (WCap IEpcc b e a) ->
+    regs !! idc = Some widc ->
+    mem !! b = Some wa ->
+    allow_jmp_mmap_or_true cond r regs mem.
+  Proof.
+    eexists IEpcc,b,e,a.
+    split ; auto.
+    unfold read_reg_inr; by simplify_map_eq.
+    case_decide; auto.
+    eexists _; by simplify_map_eq.
+  Qed.
+
+  Lemma allow_jmp_rmap_or_true_ie (cond : Prop) `{Decision cond}
+    (r : RegName) (regs : Reg)
+    (b e a : Addr) (widc : Word) :
+    regs !! r = Some (WCap IEpcc b e a) ->
+    regs !! idc = Some widc ->
+    allow_jmp_rmap_or_true cond r regs.
+  Proof.
+    eexists IEpcc,b,e,a.
+    split ; auto.
+    unfold read_reg_inr; by simplify_map_eq.
+    case_decide; auto.
+    eexists _; by simplify_map_eq.
+  Qed.
+
+  Lemma allow_jmp_mmap_or_true_ie_fail (cond : Prop) `{Decision cond}
+    (r : RegName) (regs : Reg) (mem : Mem)
+    (b e a : Addr) (widc wa wa' : Word) :
+    not (b < e)%a ->
+    regs !! r = Some (WCap IEpcc b e a) ->
+    allow_jmp_mmap_or_true cond r regs mem.
+  Proof.
+    eexists IEpcc,b,e,a.
+    split ; auto.
+    unfold read_reg_inr; by simplify_map_eq.
+    case_decide as Hajmp; auto.
+    rewrite /reg_allows_IEpcc_jmp in Hajmp.
+    by destruct Hajmp as [( _ & _ & Hcontra ) _].
+  Qed.
+
+  Lemma allow_jmp_rmap_or_true_ie_fail (cond : Prop) `{Decision cond}
+    (r : RegName) (regs : Reg)
+    (b e a : Addr) (widc wa wa' : Word) :
+    not (b < e)%a ->
+    regs !! r = Some (WCap IEpcc b e a) ->
+    allow_jmp_rmap_or_true cond r regs.
+  Proof.
+    eexists IEpcc,b,e,a.
+    split ; auto.
+    unfold read_reg_inr; by simplify_map_eq.
+    case_decide as Hajmp; auto.
+    rewrite /reg_allows_IEpcc_jmp in Hajmp.
+    by destruct Hajmp as [( _ & _ & Hcontra ) _].
+  Qed.
+
+  Lemma allow_jmp_mmap_or_true_false_cond
+    (cond : Prop) `{Decision cond} (r : RegName) (regs : Reg) (mem : Mem)
+    (p : Perm) (b e a : Addr) :
+    read_reg_inr regs r p b e a ->
+    not cond ->
+    allow_jmp_mmap_or_true cond r regs mem.
+  Proof.
+    intros Hrinr Hcond.
+    rewrite /allow_jmp_mmap_or_true.
+    eexists _,_,_,_; split ; eauto.
+    rewrite decide_False //=.
+    by intros [_ ?]; apply Hcond.
+  Qed.
+
+  Lemma allow_jmp_rmap_or_true_false_cond
+    (cond : Prop) `{Decision cond} (r : RegName) (regs : Reg)
+    (p : Perm) (b e a : Addr) :
+    read_reg_inr regs r p b e a ->
+    not cond ->
+    allow_jmp_rmap_or_true cond r regs.
+  Proof.
+    intros Hrinr Hcond.
+    rewrite /allow_jmp_rmap_or_true.
+    eexists _,_,_,_; split ; eauto.
+    rewrite decide_False //=.
+    by intros [_ ?]; apply Hcond.
+  Qed.
+
+  Definition cond_jmp : Prop := True.
+  Lemma wp_jmpIEpcc Ep pc_p pc_b pc_e pc_a r w mem regs  :
+    decodeInstrW w = JmpIEpcc r →
+    isCorrectPC (WCap pc_p pc_b pc_e pc_a) →
+
+    regs !! PC = Some (WCap pc_p pc_b pc_e pc_a) →
+    allow_jmp_mmap_or_true cond_jmp r regs mem ->
+    allow_jmp_rmap_or_true cond_jmp r regs ->
+    regs_of (JmpIEpcc r) ⊆ dom regs →
+    mem !! pc_a = Some w →
+
+    {{{ (▷ [∗ map] a↦w ∈ mem, a ↦ₐ w) ∗
+          ▷ [∗ map] k↦y ∈ regs, k ↦ᵣ y }}}
+      Instr Executable @ Ep
+      {{{ regs' retv, RET retv;
+          ⌜ Jmp_spec regs r regs' mem retv⌝ ∗
+            ([∗ map] a↦w ∈ mem, a ↦ₐ w) ∗
+            [∗ map] k↦y ∈ regs', k ↦ᵣ y }}}.
+  Proof.
+    iIntros (Hinstr Hvpc HPC Hmmap Hrmap Dregs Hmem_pc φ) "(>Hmem & >Hmap) Hφ".
+    iApply wp_lift_atomic_head_step_no_fork; auto.
+    iIntros (σ1 ns l1 l2 nt) "[Hr Hm] /=". destruct σ1; simpl.
+    iDestruct (gen_heap_valid_inclSepM with "Hr Hmap") as %Hregs.
+
+    (* Derive necessary register values in r *)
+    pose proof (lookup_weaken _ _ _ _ HPC Hregs).
+    specialize (indom_regs_incl _ _ _ Dregs Hregs) as Hri. unfold regs_of in Hri.
+    odestruct (Hri r) as [rv [Hr' _]]; first set_solver+. clear Hri.
+    (* Derive the PC in memory *)
+    iDestruct (gen_mem_valid_inSepM mem m with "Hm Hmem") as %Hma; eauto.
+
+    iModIntro.
+    iSplitR. by iPureIntro; apply normal_always_head_reducible.
+    iNext. iIntros (e2 σ2 efs Hpstep).
+    apply prim_step_exec_inv in Hpstep as (-> & -> & (c & -> & Hstep)).
+    iIntros "_".
+    iSplitR; auto. eapply step_exec_inv in Hstep; eauto.
+
+    rewrite /exec /= in Hstep.
+
+    (* Now we start splitting on the different cases in the Jmp spec, and prove them one at a time *)
+    assert (Hr0 : r0 !! r = Some rv).
+    { eapply (lookup_weaken regs r0) ;auto. }
+    destruct (is_iepcc_cap rv) eqn:Hrv.
+    - (* rv is an IEpcc-capability *)
+      destruct rv; simpl in Hrv; try discriminate.
+      destruct sb as [ p b e a |]; simpl in Hrv; try discriminate.
+      destruct p; try discriminate ; clear Hrv.
+
+      (*  destruct the bounds *)
+      destruct (decide (b <? e)%a)
+        as [Hbounds%Is_true_true | Hbounds%Is_true_false]
+      ; (rewrite Hr0 /= Hbounds /= in Hstep).
+
+      + (* in bounds, success *)
+        pose proof Hr' as Hr.
+        destruct Hmmap as (p'&b'&e'&a'& Hrinr & HallowLoad).
+        destruct Hrmap as (p''&b''&e''&a''& Hrinr' & HallowLoad').
+
+        rewrite /read_reg_inr in Hrinr, Hrinr'.
+        rewrite Hr in Hrinr, Hrinr'; symmetry in Hrinr, Hrinr' ; simplify_eq.
+
+        case_decide as Hdec ; last simplify_map_eq.
+        2: { exfalso; apply Hdec. repeat (split ; auto).
+             admit. (* TODO: easy arithmetic *)
+        }
+        destruct Hdec as [(Hreg & _ & _) _].
+        destruct HallowLoad as (wpc & HbLoad).
+        destruct HallowLoad' as (w' & Hidc).
+
+        iDestruct (gen_mem_valid_inSepM mem m b wpc with "Hm Hmem" ) as %Hma'
+        ; eauto.
+        rewrite Hma' /= in Hstep; simplify_pair_eq ; simpl.
+        iMod ((gen_heap_update_inSepM _ _ PC wpc) with "Hr Hmap") as "[Hr Hmap]"; eauto.
+        iMod ((gen_heap_update_inSepM _ _ idc (WCap RW b e a)) with "Hr Hmap") as
+          "[Hr Hmp]" ; eauto.
+        { apply lookup_insert_is_Some'; right; auto. }
+        iFrame; try iApply "Hφ"; iFrame.
+        iPureIntro; eapply Jmp_spec_success_IEpcc; eauto.
+        admit. (* TODO: easy arithmetic *)
+
+      + (* in bounds, failure *)
+        simplify_pair_eq; iFrame; iApply "Hφ"; iFrame.
+        iPureIntro; eapply Jmp_spec_failure; eauto ; first econstructor 2 ; eauto.
+        admit. (* TODO: easy arithmetic *)
+
+    - (* rv is not an IEpcc-capability, always fails *)
+      rewrite Hr0 /= in Hstep; simplify_pair_eq.
+      destruct rv; simpl in Hrv; try discriminate.
+      2: destruct sb as [ p b e a |]; simpl in Hrv; try discriminate.
+      2: destruct p; try discriminate ; clear Hrv.
+      all: simplify_pair_eq; iFrame; iApply "Hφ"; iFrame.
+      all: iPureIntro; eapply Jmp_spec_failure; eauto ; first econstructor 1 ; eauto.
+  Admitted.
+
+  (* Lemma wp_jmpIEpcc_success E pc_p pc_b pc_e pc_a w r w' : *)
+  (*   decodeInstrW w = Jmp r → *)
+  (*   isCorrectPC (WCap pc_p pc_b pc_e pc_a) → *)
+  (*   is_ie_cap w' = false -> *)
+
+  (*   {{{ ▷ PC ↦ᵣ WCap pc_p pc_b pc_e pc_a *)
+  (*         ∗ ▷ pc_a ↦ₐ w *)
+  (*         ∗ ▷ r ↦ᵣ w' }}} *)
+  (*     Instr Executable @ E *)
+  (*     {{{ RET NextIV; *)
+  (*         PC ↦ᵣ updatePcPerm w' *)
+  (*           ∗ pc_a ↦ₐ w *)
+  (*           ∗ r ↦ᵣ w' }}}. *)
+  (* Proof. *)
+  (*   iIntros (Hinstr Hvpc Hw' ϕ) "(>HPC & >Hpc_a & >Hr) Hφ". *)
+
+  (*   iDestruct (memMap_resource_1 with "Hpc_a") as "Hmem". *)
+  (*   iDestruct (map_of_regs_2 with "HPC Hr") as "[Hreg %Hr]". *)
+  (*   iApply (wp_jmp with "[$Hmem $Hreg]"); eauto ; simplify_map_eq; eauto. *)
+  (*   { by eapply allow_jmp_mmap_or_true_not_ie ; eauto; simplify_map_eq. } *)
+  (*   { by eapply allow_jmp_rmap_or_true_not_ie ; eauto; simplify_map_eq. } *)
+  (*   { by rewrite !dom_insert; set_solver+. } *)
+
+  (*   iNext. *)
+  (*   iIntros (regs retv) "(%& Hmem & Hreg)". *)
+  (*   inversion H2; simplify_map_eq. *)
+  (*   - (* Success not IE *) *)
+  (*     iExtractList "Hreg" [PC;r] as ["HPC"; "Hr"]. *)
+  (*     iDestruct (big_sepM_insert with "Hmem") as "[Hpc_a _]"; auto. *)
+  (*     iApply "Hφ" ; iFrame. *)
+  (*   - (* Failure - contradiction *) *)
+  (*     exfalso. *)
+  (*     inversion H3. *)
+  (*     rewrite (_: <[PC:=WCap pc_p pc_b pc_e pc_a]> (<[r:=w']> ∅) !! r = Some w') *)
+  (*       in H4 ; [| by simplify_map_eq]. *)
+  (*     injection H4 ; intros ->. *)
+  (*     simpl in Hw' ; congruence. *)
+  (*     Unshelve. all: eauto. *)
+  (* Qed. *)
+
+  (* Lemma wp_jmp_successPC E pc_p pc_b pc_e pc_a w : *)
+  (*   decodeInstrW w = Jmp PC → *)
+  (*    isCorrectPC (WCap pc_p pc_b pc_e pc_a) → *)
+
+  (*    {{{ ▷ PC ↦ᵣ WCap pc_p pc_b pc_e pc_a *)
+  (*        ∗ ▷ pc_a ↦ₐ w }}} *)
+  (*      Instr Executable @ E *)
+  (*      {{{ RET NextIV; *)
+  (*          PC ↦ᵣ updatePcPerm (WCap pc_p pc_b pc_e pc_a) *)
+  (*          ∗ pc_a ↦ₐ w }}}. *)
+  (* Proof. *)
+  (*   iIntros (Hinstr Hvpc ϕ) "(>HPC & >Hpc_a) Hφ". *)
+  (*   iDestruct (memMap_resource_1 with "Hpc_a") as "Hmem". *)
+  (*   iDestruct (map_of_regs_1 with "HPC") as "Hreg". *)
+  (*   iApply (wp_jmp with "[$Hmem $Hreg]"); simplify_map_eq ; eauto. *)
+  (*   { eapply allow_jmp_mmap_or_true_not_ie ; eauto; simplify_map_eq. *)
+  (*     apply isCorrectPC_nonIE in Hvpc; destruct pc_p ; auto ; done. } *)
+  (*   { eapply allow_jmp_rmap_or_true_not_ie ; eauto; simplify_map_eq. *)
+  (*     apply isCorrectPC_nonIE in Hvpc; destruct pc_p ; auto ; done. } *)
+  (*   iNext. *)
+  (*   iIntros (regs retv) "(%& Hmem & Hreg)". *)
+  (*   inversion H2; simplify_map_eq. *)
+  (*   - (* Success IE - contradiction *) *)
+  (*     inversion Hvpc ; destruct H11 ; congruence. *)
+  (*   - (* Success not IE *) *)
+  (*     iExtractList "Hreg" [PC] as ["HPC"]. *)
+  (*     iDestruct (big_sepM_insert with "Hmem") as "[Hpc_a _]"; auto. *)
+  (*     iApply "Hφ" ; iFrame. *)
+  (*   - (* Failure - contradiction *) *)
+  (*     exfalso. *)
+  (*     inversion H3. *)
+  (*     simplify_map_eq. *)
+  (*     inversion Hvpc ; destruct H10 ; congruence. *)
+  (* Qed. *)
+
+  (* TODO we need to do more cases (for _automation_), where:
+       - r = idc
+       - pc_a = a
+       - pc_a = a+1
+       - fail ?
+   *)
+  (* Lemma wp_jmp_success_IEpcc E pc_p pc_b pc_e pc_a w r b e a w' wpc widc : *)
+  (*   decodeInstrW w = JmpIEpcc r → *)
+  (*    isCorrectPC (WCap pc_p pc_b pc_e pc_a) → *)
+  (*    withinBounds b e a -> *)
+  (*    withinBounds b e (a^+1)%a -> *)
+
+  (*    {{{ ▷ PC ↦ᵣ WCap pc_p pc_b pc_e pc_a *)
+  (*        ∗ ▷ r ↦ᵣ WCap IEpcc b e a *)
+  (*        ∗ ▷ idc ↦ᵣ w' *)
+  (*        ∗ ▷ pc_a ↦ₐ w *)
+  (*        ∗ ▷ a ↦ₐ wpc *)
+  (*        ∗ ▷ (a^+1)%a ↦ₐ widc *)
+  (*    }}} *)
+  (*      Instr Executable @ E *)
+  (*      {{{ RET NextIV; *)
+  (*          PC ↦ᵣ wpc *)
+  (*        ∗ r ↦ᵣ WCap IEpcc b e a *)
+  (*        ∗ idc ↦ᵣ widc *)
+  (*        ∗ pc_a ↦ₐ w *)
+  (*        ∗ a ↦ₐ wpc *)
+  (*        ∗ (a^+1)%a ↦ₐ widc }}}. *)
+  (*   Proof. *)
+  (*   iIntros (Hinstr Hvpc Hbound_a Hbound_a' ϕ) *)
+  (*     "(>HPC  & >Hr & >Hidc & >Hpc_a & >Ha & >Ha') Hφ". *)
+
+  (*   iDestruct (address_neq with "Ha' Hpc_a") as "%Ha'". *)
+  (*   iDestruct (address_neq with "Ha Ha'") as "%Hneqa". *)
+  (*   iDestruct (memMap_resource_2ne_apply with "Hpc_a Ha") as "[Hmem %Ha]". *)
+  (*   iDestruct (big_sepM_insert with "[Ha' Hmem]") as "Hmem" ; [| iFrame |]. *)
+  (*   by simplify_map_eq. *)
+  (*   iDestruct (map_of_regs_3 with "HPC Hr Hidc") as "[Hreg %Hr']". *)
+  (*   destruct Hr' as (?&?&?). *)
+  (*   iApply (wp_jmpIEpcc with "[$Hmem $Hreg]"); eauto ; simplify_map_eq; eauto. *)
+  (*   { eapply (allow_jmp_mmap_or_true_ie _ _ _ _ _ _ a); simplify_map_eq; eauto. } *)
+  (*   { by eapply allow_jmp_rmap_or_true_ie ; simplify_map_eq ; auto. } *)
+  (*   { by rewrite !dom_insert; set_solver+. } *)
+
+  (*   iNext. *)
+  (*   iIntros (regs retv) "(%Hspec& Hmem & Hreg)". *)
+  (*   inversion Hspec as [| Hfail]; simplify_map_eq. *)
+  (*   - (* Success IEpcc *) *)
+  (*     iApply "Hφ". *)
+  (*     iExtractList "Hreg" [PC;idc;r] as ["HPC"; "Hidc" ; "Hr"]. *)
+  (*     iDestruct (big_sepM_insert with "Hmem") as "[Ha' Hmem]"; auto ; [ by simplify_map_eq|]. *)
+  (*     iDestruct (big_sepM_insert with "Hmem") as "[Hpc_a Hmem]"; auto ; [ by simplify_map_eq|]. *)
+  (*     iDestruct (big_sepM_insert with "Hmem") as "[Ha _]"; auto. *)
+  (*     iFrame. *)
+  (*   - (* Failure - contradiction *) *)
+  (*     exfalso. *)
+  (*     inversion Hfail as [? Hcontra |? ? ? ? Hcontra]; simplify_map_eq. *)
+  (*     by apply Hcontra. *)
+  (* Qed. *)
+
+  (* Lemma wp_jmp_success_IEpcc_idc E pc_p pc_b pc_e pc_a w b e a wpc widc : *)
+  (*   decodeInstrW w = JmpIEpcc idc → *)
+  (*    isCorrectPC (WCap pc_p pc_b pc_e pc_a) → *)
+  (*    withinBounds b e a -> *)
+  (*    withinBounds b e (a^+1)%a -> *)
+
+  (*    {{{ ▷ PC ↦ᵣ WCap pc_p pc_b pc_e pc_a *)
+  (*        ∗ ▷ idc ↦ᵣ WCap IEpcc b e a *)
+  (*        ∗ ▷ pc_a ↦ₐ w *)
+  (*        ∗ ▷ a ↦ₐ wpc *)
+  (*        ∗ ▷ (a^+1)%a ↦ₐ widc *)
+  (*    }}} *)
+  (*      Instr Executable @ E *)
+  (*      {{{ RET NextIV; *)
+  (*          PC ↦ᵣ wpc *)
+  (*        ∗ idc ↦ᵣ widc *)
+  (*        ∗ pc_a ↦ₐ w *)
+  (*        ∗ a ↦ₐ wpc *)
+  (*        ∗ (a^+1)%a ↦ₐ widc }}}. *)
+  (*   Proof. *)
+  (*   iIntros (Hinstr Hvpc Hbound_a Hbound_a' ϕ) *)
+  (*     "(>HPC  & >Hidc & >Hpc_a & >Ha & >Ha') Hφ". *)
+
+  (*   iDestruct (address_neq with "Ha' Hpc_a") as "%Ha'". *)
+  (*   iDestruct (address_neq with "Ha Ha'") as "%Hneqa". *)
+  (*   iDestruct (memMap_resource_2ne_apply with "Hpc_a Ha") as "[Hmem %Ha]". *)
+  (*   iDestruct (big_sepM_insert with "[Ha' Hmem]") as "Hmem" ; [| iFrame |]. *)
+  (*   by simplify_map_eq. *)
+  (*   iDestruct (map_of_regs_2 with "HPC Hidc") as "[Hreg _]". *)
+  (*   iApply (wp_jmpIEpcc with "[$Hmem $Hreg]"); eauto ; simplify_map_eq; eauto. *)
+  (*   { eapply (allow_jmp_mmap_or_true_ie _ _ _ _ _ _ a) ; simplify_map_eq ; eauto. } *)
+  (*   { by eapply allow_jmp_rmap_or_true_ie ; simplify_map_eq ; auto. } *)
+  (*   { by rewrite !dom_insert; set_solver+. } *)
+
+  (*   iNext. *)
+  (*   iIntros (regs retv) "(%Hspec& Hmem & Hreg)". *)
+  (*   inversion Hspec as [| Hfail ]; simplify_map_eq. *)
+  (*   - (* Success IEpcc *) *)
+  (*     iApply "Hφ". *)
+  (*     iExtractList "Hreg" [PC;idc] as ["HPC"; "Hidc"]. *)
+  (*     iDestruct (big_sepM_insert with "Hmem") as "[Ha' Hmem]"; auto ; [ by simplify_map_eq|]. *)
+  (*     iDestruct (big_sepM_insert with "Hmem") as "[Hpc_a Hmem]"; auto ; [ by simplify_map_eq|]. *)
+  (*     iDestruct (big_sepM_insert with "Hmem") as "[Ha _]"; auto. *)
+  (*     iFrame. *)
+  (*   - (* Failure - contradiction *) *)
+  (*     exfalso. *)
+  (*     inversion Hfail as [ ? Hcontra |? ? ? ? Hcontra]; simplify_map_eq. *)
+  (*     by apply Hcontra. *)
+  (* Qed. *)
+
+  (* Lemma wp_jmp_fail_IEpcc E pc_p pc_b pc_e pc_a w r b e a : *)
+  (*   decodeInstrW w = JmpIEpcc r → *)
+  (*   isCorrectPC (WCap pc_p pc_b pc_e pc_a) → *)
+  (*   not (withinBounds b e a /\ withinBounds b e (a^+1)%a) -> *)
+
+  (*   {{{ ▷ PC ↦ᵣ WCap pc_p pc_b pc_e pc_a *)
+  (*         ∗ ▷ r ↦ᵣ WCap IEpcc b e a *)
+  (*         ∗ ▷ pc_a ↦ₐ w *)
+  (*   }}} *)
+  (*     Instr Executable @ E *)
+  (*     {{{ RET FailedV; *)
+  (*         PC ↦ᵣ WCap pc_p pc_b pc_e pc_a *)
+  (*         ∗ r ↦ᵣ WCap IEpcc b e a *)
+  (*         ∗ pc_a ↦ₐ w *)
+  (*     }}}. *)
+  (* Proof. *)
+  (*   iIntros (Hinstr Hvpc Hbounds ϕ) *)
+  (*     "(>HPC & >Hr & >Hpc_a) Hφ". *)
+
+  (*   iDestruct (memMap_resource_1 with "Hpc_a") as "Hmem". *)
+  (*   iDestruct (map_of_regs_2 with "HPC Hr") as "[Hreg %Hr']". *)
+
+  (*   iApply (wp_jmpIEpcc with "[$Hmem $Hreg]"); eauto ; simplify_map_eq; eauto. *)
+  (*   { by eapply allow_jmp_mmap_or_true_ie_fail ; simplify_map_eq ; eauto. } *)
+  (*   { by eapply allow_jmp_rmap_or_true_ie_fail ; simplify_map_eq ; eauto. } *)
+  (*   { by rewrite !dom_insert; set_solver+. } *)
+
+  (*   iNext. *)
+  (*   iIntros (regs retv) "(%Hspec& Hmem & Hreg)". *)
+  (*   inversion Hspec as [ | Hfail]; simplify_map_eq. *)
+  (*   (* Failure - contradiction *) *)
+  (*   iApply "Hφ". *)
+  (*   inversion Hfail as [? Hcontra | ? ? ? ? Hcontra ] ; simplify_map_eq. *)
+  (*   iExtractList "Hreg" [PC;r] as ["HPC"; "Hr"]. *)
+  (*   iDestruct (memMap_resource_1 with "Hmem") as "Hpc_a". *)
+  (*   iFrame. *)
+  (* Qed. *)
+
+  (* Lemma wp_jmp_success_IEpcc_same_idc E pc_p pc_b pc_e pc_a w b e a wpc widc : *)
+  (*   decodeInstrW w = JmpIEpcc idc → *)
+  (*   isCorrectPC (WCap pc_p pc_b pc_e pc_a) → *)
+  (*   withinBounds b e a -> *)
+  (*   withinBounds b e (a^+1)%a -> *)
+
+  (*   {{{ ▷ PC ↦ᵣ WCap pc_p pc_b pc_e pc_a *)
+  (*         ∗ ▷ idc ↦ᵣ WCap IEpcc b e a *)
+  (*         ∗ ▷ pc_a ↦ₐ w *)
+  (*         ∗ ▷ a ↦ₐ wpc *)
+  (*         ∗ ▷ (a^+1)%a ↦ₐ widc *)
+  (*   }}} *)
+  (*     Instr Executable @ E *)
+  (*     {{{ RET NextIV; *)
+  (*         PC ↦ᵣ wpc *)
+  (*           ∗ idc ↦ᵣ widc *)
+  (*           ∗ pc_a ↦ₐ w *)
+  (*           ∗ a ↦ₐ wpc *)
+  (*           ∗ (a^+1)%a ↦ₐ widc }}}. *)
+  (* Proof. *)
+  (*   iIntros (Hinstr Hvpc Hbound_a Hbound_a' ϕ) *)
+  (*     "(>HPC & >Hidc & >Hpc_a & >Ha & >Ha') Hφ". *)
+
+  (*   iDestruct (address_neq with "Ha' Hpc_a") as "%Ha'". *)
+  (*   iDestruct (address_neq with "Ha Ha'") as "%Hneqa". *)
+  (*   iDestruct (memMap_resource_2ne_apply with "Hpc_a Ha") as "[Hmem %Ha]". *)
+  (*   iDestruct (big_sepM_insert with "[Ha' Hmem]") as "Hmem" ; [| iFrame |]. *)
+  (*   by simplify_map_eq. *)
+  (*   iDestruct (map_of_regs_2 with "HPC Hidc") as "[Hreg %Hr']". *)
+  (*   iApply (wp_jmpIEpcc with "[$Hmem $Hreg]"); eauto ; simplify_map_eq; eauto. *)
+  (*   { eapply (allow_jmp_mmap_or_true_ie _ _ _ _ _ _ a) ; simplify_map_eq ; eauto. } *)
+  (*   { by eapply allow_jmp_rmap_or_true_ie ; simplify_map_eq ; auto. } *)
+  (*   { by rewrite !dom_insert; set_solver+. } *)
+
+  (*   iNext. *)
+  (*   iIntros (regs retv) "(%Hspec& Hmem & Hreg)". *)
+  (*   inversion Hspec as [ | Hfail]; simplify_map_eq. *)
+  (*   - (* Success IE *) *)
+  (*     iApply "Hφ". *)
+  (*     iExtractList "Hreg" [PC;idc] as ["HPC"; "Hidc"]. *)
+  (*     iDestruct (big_sepM_insert with "Hmem") as "[Ha' Hmem]"; auto ; [ by simplify_map_eq|]. *)
+  (*     iDestruct (big_sepM_insert with "Hmem") as "[Hpc_a Hmem]"; auto ; [ by simplify_map_eq|]. *)
+  (*     iDestruct (big_sepM_insert with "Hmem") as "[Ha _]"; auto. *)
+  (*     iFrame. *)
+  (*   - (* Failure - contradiction *) *)
+  (*     exfalso. *)
+  (*     inversion Hfail as [ ? Hcontra | ? ? ? ? Hcontra ]; simplify_map_eq. *)
+  (*     by apply Hcontra. *)
+  (* Qed. *)
+
+  (* Lemma wp_jmp_fail_IEpcc_same_idc E pc_p pc_b pc_e pc_a w b e a : *)
+  (*   decodeInstrW w = JmpIEpcc idc → *)
+  (*   isCorrectPC (WCap pc_p pc_b pc_e pc_a) → *)
+  (*   not (withinBounds b e a /\ withinBounds b e (a^+1)%a) -> *)
+
+  (*   {{{ ▷ PC ↦ᵣ WCap pc_p pc_b pc_e pc_a *)
+  (*         ∗ ▷ idc ↦ᵣ WCap IEpcc b e a *)
+  (*         ∗ ▷ pc_a ↦ₐ w *)
+  (*   }}} *)
+  (*     Instr Executable @ E *)
+  (*     {{{ RET FailedV; *)
+  (*         PC ↦ᵣ WCap pc_p pc_b pc_e pc_a *)
+  (*           ∗ idc ↦ᵣ WCap IEpcc b e a *)
+  (*           ∗ pc_a ↦ₐ w *)
+  (*     }}}. *)
+  (* Proof. *)
+  (*   iIntros (Hinstr Hvpc Hbounds ϕ) *)
+  (*     "(>HPC & >Hidc & >Hpc_a) Hφ". *)
+
+  (*   iDestruct (map_of_regs_2 with "HPC Hidc") as "[Hreg %Hr']". *)
+  (*   iDestruct (memMap_resource_1 with "Hpc_a") as "Hmem". *)
+
+  (*   iApply (wp_jmpIEpcc with "[$Hmem $Hreg]"); eauto ; simplify_map_eq; eauto. *)
+  (*   { by eapply allow_jmp_mmap_or_true_ie_fail ; simplify_map_eq ; eauto. } *)
+  (*   { by eapply allow_jmp_rmap_or_true_ie_fail ; simplify_map_eq ; eauto. } *)
+  (*   { by rewrite !dom_insert; set_solver+. } *)
+
+  (*   iNext. *)
+  (*   iIntros (regs retv) "(%Hspec& Hmem & Hreg)". *)
+  (*   inversion Hspec as [ | Hfail]; simplify_map_eq. *)
+  (*   (* Failure - contradiction *) *)
+  (*   iApply "Hφ". *)
+  (*   inversion Hfail as [ ? Hcontra | ? ? ? ? Hcontra ] ; simplify_map_eq. *)
+  (*   iExtractList "Hreg" [PC;idc] as ["HPC"; "Hidc"]. *)
+  (*   iDestruct (memMap_resource_1 with "Hmem") as "Hpc_a". *)
+  (*   iFrame. *)
+  (* Qed. *)
+
+End cap_lang_rules.
